\section{Newton Interpolating Polynomials}

The general newton interpolating polynomial can be expressed as:
\begin{equation}
f_n(x) = b_0 + b_1(x-x_0) + \dots + b_n(x-x_0) \dots (x-x_{n-1})
\end{equation}

or in summation form as:

\begin{equation}
f_n(x) = b_0 + \sum_{i=1}^{i<n} b_i \prod_{j=0}^{j<i} (x-x_j)
\end{equation}

We can build an upper triangular matrix, where the diagonal of the matrix will be the coefficient $b_i$

\gbox{
	A_{i,j} = \frac{b_{i-1,j} - b_{i-1,j-1}}{x_j-x_{j-i-1}}
	\quad
	(0 \leq i < n)
	(0 \leq j < i)
}
